chapter06-refine/exercises/impl_model_for_ex04.dfy
@@ -1,4 +1,14 @@
-//#desc Given model for exercise03
+//#desc Implementation state machine for refinement proof in exercise04.
+
+// This file is an instructor-supplied solution to the 2PC implementation in
+// chapter 5, so you're not doing battle with an implementation that's
+// impossible to prove. In fact, you can reuse parts of the instructor-supplied
+// proof from here as well.
+//
+
+// TODO(manos): how should we ensure this file is disseminated at the
+// appropriate time, so students aren't waiting for it?
+
 // This file is an "official solution" to exercises 01 & 02, to ensure you're
 // not doing battle with mistakes in your own protocol definition.  The proof
 // is challenging enough for an exercise without fighting protocol bugs.
@@ -528,5 +538,104 @@ module Obligations {
     && SafetyAC1(c, v)
     && SafetyAC3(c, v)
     && SafetyAC4(c, v)
+  }
+}
+
+module TwoPCInvariantProof {
+  import opened CommitTypes
+  import opened Types
+  import opened Library
+  import opened DistributedSystem
+  import opened Obligations
+
+  predicate VoteMessagesAgreeWithParticipantPreferences(c: Constants, v: Variables)
+    requires v.WF(c)
+  {
+    (forall msg |
+      && msg in v.network.sentMsgs
+      && msg.VoteMsg?
+      && ValidParticipantId(c, msg.sender)
+      :: msg.vote == ParticipantConstants(c, msg.sender).preference
+    )
+  }
+
+  predicate CoordinatorStateSupportedByVote(c: Constants, v: Variables)
+    requires v.WF(c)
+  {
+    (forall idx:HostId |
+      && ValidParticipantId(c, idx)
+      && CoordinatorVars(c, v).votes[idx].Some?
+      :: VoteMsg(idx, CoordinatorVars(c, v).votes[idx].value) in v.network.sentMsgs
+    )
+  }
+
+  predicate DecisionMsgsAgreeWithDecision(c: Constants, v: Variables)
+    requires v.WF(c)
+  {
+    (forall msg |
+      && msg in v.network.sentMsgs
+      && msg.DecisionMsg?
+      :: CoordinatorHost.ObservesResult(CoordinatorConstants(c), CoordinatorVars(c, v), msg.decision)
+    )
+  }
+
+  predicate Inv(c: Constants, v: Variables)
+  {
+    && v.WF(c)
+    && VoteMessagesAgreeWithParticipantPreferences(c, v)
+    && CoordinatorStateSupportedByVote(c, v)
+    // We'll give you one invariant to get you started...
+    && DecisionMsgsAgreeWithDecision(c, v)
+    // ...but you'll need more.
+    && Safety(c, v)
+  }
+
+  lemma InitImpliesInv(c: Constants, v: Variables)
+    requires Init(c, v)
+    ensures Inv(c, v)
+  {
+    // Nobody has agreed with anything yet, so they agree with both.
+    assert AllWithDecisionAgreeWithThisOne(c, v, Commit); // witness.
+    assert AllWithDecisionAgreeWithThisOne(c, v, Abort); // witness.
+  }
+
+  lemma InvInductive(c: Constants, v: Variables, v': Variables)
+    requires Inv(c, v)
+    requires Next(c, v, v')
+    ensures Inv(c, v')
+  {
+    // The body of this lemma got really big (expanding foralls, case splits,
+    // testing asserts) while I was figuring out what invariants were missing
+    // ... and fixing a couple of errors in the protocol definition itself.
+    // Afterward, nearly all of that text could be deleted.
+
+    var step :| NextStep(c, v, v', step);   // Witness
+
+    // sklomize msg from DecisionMsgsAgreeWithDecision
+    forall msg |
+      && msg in v'.network.sentMsgs
+      && msg.DecisionMsg?
+      ensures CoordinatorHost.ObservesResult(CoordinatorConstants(c), CoordinatorVars(c, v'), msg.decision)
+    {
+      var hostid := step.hostid;
+      assert Host.Next(c.hosts[hostid], v.hosts[hostid], v'.hosts[hostid], step.msgOps);  // observe trigger
+      if msg in v.network.sentMsgs {  // observe trigger
+//        assert CoordinatorHost.ObservesResult(CoordinatorConstants(c), CoordinatorVars(c, v), msg.decision);
+//        assert CoordinatorHost.AllVotesCollected(CoordinatorConstants(c), CoordinatorVars(c,v'));
+        // trigger: hey, all the votes are the same!
+        // wait why is that true? That's not true when receiving a vote. Hrm.
+        assert forall hostIdx:HostId | hostIdx < |CoordinatorVars(c,v).votes| :: CoordinatorVars(c,v').votes[hostIdx] == CoordinatorVars(c,v).votes[hostIdx];
+//        assert CoordinatorHost.ObservesResult(CoordinatorConstants(c), CoordinatorVars(c, v'), msg.decision);
+//      } else {
+
+      }
+    }
+//    assert Safety(c, v'); // somehow this trigger is necessary to get the forall above! Bizarre.
+  }
+
+  lemma InvImpliesSafety(c: Constants, v: Variables)
+    requires Inv(c, v)
+    ensures Safety(c, v)
+  { // Trivial, as usual, since safety is a conjunct in Inv.
   }
 }
