chapter06-refine/exercises/exercise04.dfy
@@ -1,0 +1,284 @@
+//#title Refinement proof for 2PC
+//#desc Show that Two Phase Commit refines the Atomic Commit sate machine spec.
+
+// This proof shouldn't be terribly brutal, since you have a roadmap for the
+// relevant invariants from chapter05. You can discard the AC properties (since
+// those are proven about the spec in exercise03, and therefore about any state
+// machine that refines the spec).
+
+include "spec_model_for_ex04.dfy"
+include "impl_model_for_ex04.dfy"
+
+// This Dafny "abstract module" establishes the proof obligations for the refinement:
+// you must fill in the function and lemma bodies in a module that `refines` this one.
+// So leave this module as-is, and fill in the bodies in the refining module.
+// (This structure isn't necessary, but it's a nice way to separate the statement
+// of the theorem from its proof.)
+abstract module RefinementTheorem {
+  import opened CommitTypes
+  import opened Types
+  import opened Library
+  import opened DistributedSystem
+  import opened TwoPCInvariantProof
+  import AtomicCommit
+
+  function ConstantsAbstraction(c: DistributedSystem.Constants) : AtomicCommit.Constants
+    requires c.WF()
+
+  function VariablesAbstraction(c: DistributedSystem.Constants, v: DistributedSystem.Variables) : AtomicCommit.Variables
+    requires v.WF(c)
+
+  predicate Inv(c: DistributedSystem.Constants, v: DistributedSystem.Variables)
+
+  lemma RefinementInit(c: DistributedSystem.Constants, v: DistributedSystem.Variables)
+    requires DistributedSystem.Init(c, v)
+    ensures Inv(c, v)
+    ensures AtomicCommit.Init(ConstantsAbstraction(c), VariablesAbstraction(c, v))
+
+  lemma RefinementNext(c: DistributedSystem.Constants, v: DistributedSystem.Variables, v': DistributedSystem.Variables)
+    requires DistributedSystem.Next(c, v, v')
+    requires Inv(c, v)
+    ensures Inv(c, v')
+    ensures AtomicCommit.Next(ConstantsAbstraction(c), VariablesAbstraction(c, v), VariablesAbstraction(c, v')) || VariablesAbstraction(c, v) == VariablesAbstraction(c, v')
+
+}
+
+module RefinementProof refines RefinementTheorem {
+  // No imports needed because we inherited them from the abstract module RefinementTheorem
+  import opened Obligations
+  import opened CoordinatorHost
+
+  function ParticipantCount(c: DistributedSystem.Constants) : nat
+    requires c.WF()
+  {
+    CoordinatorConstants(c).participantCount
+  }
+
+  function ConstantsAbstraction(c: DistributedSystem.Constants) : AtomicCommit.Constants
+  {
+    AtomicCommit.Constants(ParticipantCount(c),
+      seq(ParticipantCount(c), idx requires 0 <= idx < ParticipantCount(c) => ParticipantConstants(c, idx).preference))
+  }
+
+  function VariablesAbstraction(c: DistributedSystem.Constants, v: DistributedSystem.Variables) : AtomicCommit.Variables
+  {
+    AtomicCommit.Variables(CoordinatorVars(c, v).decision,
+      seq(ParticipantCount(c), idx requires 0 <= idx < ParticipantCount(c) => ParticipantVars(c, v, idx).decision))
+  }
+
+/*
+  predicate VoteMessagesAgreeWithParticipantPreferences(c: DistributedSystem.Constants, v: DistributedSystem.Variables)
+    requires v.WF(c)
+  {
+    (forall msg |
+      && msg in v.network.sentMsgs
+      && msg.VoteMsg?
+      && ValidParticipantId(c, msg.sender)
+      :: msg.vote == ParticipantConstants(c, msg.sender).preference
+    )
+  }
+
+  predicate CoordinatorStateSupportedByVote(c: DistributedSystem.Constants, v: DistributedSystem.Variables)
+    requires c.WF()
+    requires v.WF(c)
+  {
+    (forall idx:ParticipantId |
+      && c.ValidParticipantId(idx)
+      && v.coordinator.votes[idx].Some?
+      :: VoteMsg(idx, v.coordinator.votes[idx].value) in v.network.sentMsgs
+    )
+  }
+
+  predicate DecisionMsgsAgreeWithDecision(c: DistributedSystem.Constants, v: DistributedSystem.Variables)
+    requires c.WF()
+    requires v.WF(c)
+  {
+    (forall msg |
+      && msg in v.network.sentMsgs
+      && msg.DecisionMsg?
+      :: CoordinatorHost.ObservesResult(c.coordinator, v.coordinator, msg.decision)
+    )
+  }
+*/
+
+  predicate Inv(c: DistributedSystem.Constants, v: DistributedSystem.Variables)
+  {
+  /*
+    && c.WF()
+    && v.WF(c)
+    && VoteMessagesAgreeWithParticipantPreferences(c, v)
+    && CoordinatorStateSupportedByVote(c, v)
+    && DecisionMsgsAgreeWithDecision(c, v)
+    */
+    && TwoPCInvariantProof.Inv(c, v)
+  }
+
+  lemma RefinementInit(c: DistributedSystem.Constants, v: DistributedSystem.Variables)
+    /*
+    requires DistributedSystem.Init(c, v)
+    ensures Inv(c, v)
+    ensures AtomicCommit.Init(ConstantsAbstraction(c), VariablesAbstraction(c, v))*/
+  {
+    assert Inv(c, v);
+    assert AtomicCommit.Init(ConstantsAbstraction(c), VariablesAbstraction(c, v));
+  }
+
+  lemma RefinementNext(c: DistributedSystem.Constants, v: DistributedSystem.Variables, v': DistributedSystem.Variables)
+    /*requires DistributedSystem.Next(c, v, v')
+    requires Inv(c, v)
+    ensures Inv(c, v')
+    ensures AtomicCommit.Next(ConstantsAbstraction(c), VariablesAbstraction(c, v), VariablesAbstraction(c, v')) || VariablesAbstraction(c, v) == VariablesAbstraction(c, v')*/
+  {
+    assert Inv(c, v);
+    assert DistributedSystem.Next(c, v, v');
+    InvInductive(c, v, v'); // Reuse this from chapter05/exercises/exercise03 proof
+    assert Inv(c, v');
+
+    // Skolemize the DistributedSystem step (learn which step we need to
+    // consider), and case split on type of the host that stepped (Coordinator
+    // or Participant).
+    var step :| DistributedSystem.NextStep(c, v, v', step);
+    var hc := c.hosts[step.hostid];
+    match hc {
+      case CoordinatorConstants(_) => {
+        // Skolemize the CoordinatorHost step that happened, and case split on it.
+        var hstep :| CoordinatorHost.NextStep(CoordinatorConstants(c), CoordinatorVars(c, v), CoordinatorVars(c, v'), hstep, step.msgOps);
+        match hstep {
+          case SendReqStep => {
+            assert VariablesAbstraction(c, v) == VariablesAbstraction(c, v');
+          }
+          case LearnVoteStep => {
+            assert VariablesAbstraction(c, v) == VariablesAbstraction(c, v');
+          }
+          case DecideStep(decision) => {
+            if CoordinatorVars(c, v).decision.Some? {
+              // If coordinator had already decided, then this step is (had better be) a noop, because
+              // we didn't change the decision.
+              assert VariablesAbstraction(c, v) == VariablesAbstraction(c, v');
+            } else {
+              // Coordinator made a decision; provide a witness to that step in the AtomicCommit machine
+              assert CoordinatorVars(c, v).WF(CoordinatorConstants(c));
+              assert |v.hosts|-1 == CoordinatorConstants(c).participantCount;
+              assert |CoordinatorVars(c, v).votes| == |v.hosts|-1;
+              assert forall hostIdx:HostId | hostIdx < ParticipantCount(c) :: CoordinatorVars(c, v').votes[hostIdx].value
+                == ParticipantConstants(c, hostIdx).preference;
+              if (forall hostIdx:HostId | hostIdx < ParticipantCount(c) :: CoordinatorVars(c, v').votes[hostIdx].value.Yes?) {
+                assert CoordinatorVars(c, v').decision.value.Commit?;
+              } else {
+                assert CoordinatorVars(c, v').decision.value.Abort?;
+              }
+              assert ConstantsAbstraction(c).participantCount == ParticipantCount(c);
+              assert forall idx:HostId :: ConstantsAbstraction(c).ValidParticipant(idx) == (idx < ParticipantCount(c));
+              if (forall hostIdx:HostId | hostIdx < ParticipantCount(c) :: ParticipantConstants(c, hostIdx).preference.Yes?) {
+                assert AtomicCommit.UltimateDecision(ConstantsAbstraction(c)).Commit?;
+              } else {
+                assert AtomicCommit.UltimateDecision(ConstantsAbstraction(c)).Abort?;
+              }
+              assert CoordinatorVars(c, v').decision.value == AtomicCommit.UltimateDecision(ConstantsAbstraction(c));
+              assert AtomicCommit.NextStep(ConstantsAbstraction(c), VariablesAbstraction(c, v), VariablesAbstraction(c, v'), AtomicCommit.CoordinatorLearnsStep);
+              assert AtomicCommit.Next(ConstantsAbstraction(c), VariablesAbstraction(c, v), VariablesAbstraction(c, v'));
+            }
+          }
+        }
+        assert AtomicCommit.Next(ConstantsAbstraction(c), VariablesAbstraction(c, v), VariablesAbstraction(c, v')) || VariablesAbstraction(c, v) == VariablesAbstraction(c, v');
+      }
+      case ParticipantConstants(_) => {
+        assert AtomicCommit.Next(ConstantsAbstraction(c), VariablesAbstraction(c, v), VariablesAbstraction(c, v')) || VariablesAbstraction(c, v) == VariablesAbstraction(c, v');
+      }
+    }
+    assert AtomicCommit.Next(ConstantsAbstraction(c), VariablesAbstraction(c, v), VariablesAbstraction(c, v')) || VariablesAbstraction(c, v) == VariablesAbstraction(c, v');
+
+//    assert forall idx:AtomicCommit.ParticipantId :: ConstantsAbstraction(c).ValidParticipant(idx) == ValidParticipantId(c, idx);
+//
+//    var step :| DistributedSystem.NextStep(c, v, v', step);
+//    var hc := c.hosts[step.hostid];
+//    match hc {
+//      case CoordinatorConstants => {
+//        assert DecisionMsgsAgreeWithDecision(c, v'); // Trigger
+//        //if VariablesAbstraction(c, v) == VariablesAbstraction(c, v') {
+//        assert Coordinator(c, v, v', msgOps);
+//        assert CoordinatorHost.Next(c.coordinator, v.coordinator, v'.coordinator, msgOps);
+//        assert (forall idx:nat | c.ValidParticipantId(idx) :: v'.participants[idx] == v.participants[idx]);
+//
+//        //assert exists step2 :: CoordinatorHost.NextStep(c.coordinator, v.coordinator, v'.coordinator, step2, msgOps);
+//        var coordinatorStep :| CoordinatorHost.NextStep(c.coordinator, v.coordinator, v'.coordinator, coordinatorStep, msgOps);
+//        match coordinatorStep {
+//          case SendReqStep() => {
+//            assert SendReq(c.coordinator, v.coordinator, v'.coordinator, msgOps);
+//            assert v.coordinator == v'.coordinator;
+//            assert VariablesAbstraction(c, v) == VariablesAbstraction(c, v');
+//            //assert v == v';
+//            //assert AtomicCommit.Next(ConstantsAbstraction(c), VariablesAbstraction(c, v), VariablesAbstraction(c, v'));
+//          }
+//          case LearnVoteStep() => {
+//            assert LearnVote(c.coordinator, v.coordinator, v'.coordinator, msgOps);
+//            assert VariablesAbstraction(c, v) == VariablesAbstraction(c, v');
+//            //assert AtomicCommit.Next(ConstantsAbstraction(c), VariablesAbstraction(c, v), VariablesAbstraction(c, v'));
+//          }
+//          case DecideStep(decision) => {
+//            assert Decide(c.coordinator, v.coordinator, v'.coordinator, decision, msgOps);
+//            if(v.coordinator.decision.None?) {
+//              //assume false;
+//              assert v'.coordinator.decision.Some?;
+//              var decision := v'.coordinator.decision.value;
+//              assert ObservesResult(c.coordinator, v.coordinator, decision);
+//              var abs := ConstantsAbstraction(c);
+//
+//              /*calc {
+//                  AtomicCommit.UltimateDecision(ConstantsAbstraction(c)).Commit?;
+//                  forall idx:ParticipantId | ConstantsAbstraction(c).ValidParticipant(idx) :: ConstantsAbstraction(c).preferences[idx] == Yes;
+//                  {
+//                    //
+//                    //assert forall idx:ParticipantId | ConstantsAbstraction(c).ValidParticipant(idx) :: c.participants[idx].preference.Yes? == ConstantsAbstraction(c).preferences[idx].Yes?;
+//                    }
+//
+//                  forall hostIdx:ParticipantId | c.coordinator.ValidParticipantId(hostIdx) :: c.participants[hostIdx].preference.Yes?;
+//                  forall hostIdx:ParticipantId | c.coordinator.ValidParticipantId(hostIdx) :: v.coordinator.votes[hostIdx].value.Yes?;
+//                  decision.Commit?;
+//              }
+//
+//              if (forall hostIdx:ParticipantId | c.coordinator.ValidParticipantId(hostIdx) :: v.coordinator.votes[hostIdx].value.Yes?) {
+//                //assert forall idx |
+//                assert decision == Commit;
+//                //assert forall idx | 0 <= idx < |c.coordinator.participants| ==> abs.
+//
+//                assert decision == AtomicCommit.UltimateDecision(ConstantsAbstraction(c));
+//
+//              } else {
+//                assert decision == Abort;
+//                assert decision == AtomicCommit.UltimateDecision(ConstantsAbstraction(c));
+//              }*/
+//
+//              //assert AtomicCommit.CoordinatorLearnsDecision(ConstantsAbstraction(c), VariablesAbstraction(c, v), VariablesAbstraction(c, v'));
+//              assert AtomicCommit.NextStep(ConstantsAbstraction(c), VariablesAbstraction(c, v), VariablesAbstraction(c, v'), AtomicCommit.CoordinatorLearnsStep());
+//              //assert AtomicCommit.Next(ConstantsAbstraction(c), VariablesAbstraction(c, v), VariablesAbstraction(c, v'));
+//            } else {
+//              assert VariablesAbstraction(c, v) == VariablesAbstraction(c, v');
+//            }
+//          }
+//        }
+//
+//        assert AtomicCommit.Next(ConstantsAbstraction(c), VariablesAbstraction(c, v), VariablesAbstraction(c, v')) || VariablesAbstraction(c, v) == VariablesAbstraction(c, v');
+//        //}
+//      }
+//      case ParticipantConstants => {
+//        assert Inv(c, v');
+//
+//        assume AtomicCommit.Next(ConstantsAbstraction(c), VariablesAbstraction(c, v), VariablesAbstraction(c, v')) || VariablesAbstraction(c, v) == VariablesAbstraction(c, v');
+//        /*if v != v' {
+//          assume AtomicCommit.Next(ConstantsAbstraction(c), VariablesAbstraction(c, v), VariablesAbstraction(c, v'));
+//        } */
+//      }
+//    }
+//    assert Inv(c, v');
+//
+//    //assume AtomicCommit.Next(ConstantsAbstraction(c), VariablesAbstraction(c, v), VariablesAbstraction(c, v')) || v == v';
+//
+//    /*
+//    if (v != v') {
+//      var step :| DistributedSystem.NextStep(c, v, v', step);
+//
+//    }*/
+//    //assert AtomicCommit.Next(ConstantsAbstraction(c), VariablesAbstraction(c, v), VariablesAbstraction(c, v'));
+  }
+}
